ChoiceAlgebra/theories/ChoiceAlgebra.v
@@ -73,11 +73,15 @@ End ChoiceAlgebraLemmas.
     Total operations come from Resource.v; definedness remains explicit in
     [ca_times_def] and [ca_plus_def]. *)
 
-#[global] Program Instance WfWorld_ChoiceAlgebra : ChoiceAlgebra WfWorld := {|
+Section WfWorldChoiceAlgebra.
+
+Context {V : Type} `{ValueSig V}.
+
+#[global] Program Instance WfWorld_ChoiceAlgebra : ChoiceAlgebra (WfWorld (V := V)) := {|
   ca_one       := res_unit;
   ca_times     := res_product_total;
   ca_plus      := res_sum_total;
-  ca_le        := sqsubseteq (A := WfWorld);
+  ca_le        := sqsubseteq (A := WfWorld (V := V));
   ca_times_def := fun w1 w2 => world_compat w1 w2;
   ca_plus_def  := fun w1 w2 => raw_sum_defined w1 w2;
 |}.
@@ -91,3 +95,5 @@ Next Obligation.                 (* ca_le_refl: provable because carrier is WfWo
 Qed.
 Next Obligation. Admitted.       (* ca_times_le_mono *)
 Next Obligation. Admitted.       (* ca_plus_le_mono *)
+
+End WfWorldChoiceAlgebra.
